Steel.ListP

steel/Learn.Steel.ListP.Data.fst
@@ -11,7 +11,7 @@ open Learn.Steel.ListP.Param
 
 
 let mlist_cons_sel (p : list_param) (entry : ref p.r) (len' : nat) (exit : ref p.r)
-                   (sels : (c : t_of (p.cell entry).vp
+                   (sels : (c : t_of (vcell p entry)
                               & mlist_sel_t p ((p.cell entry).get_next c) len' exit))
   : GTot (mlist_sel_t p entry (len'+1) exit)
   = let (|c, rs|) = sels in (|entry, (p.cell entry).get_data c|) :: rs
@@ -22,10 +22,10 @@ let rec mlist0 (p : list_param) (entry : ref p.r) (len : nat) (exit : ref p.r)
   =
     if len = 0
     then vrewrite (US.pure (entry == exit)) #(mlist_sel_t p entry len exit) (fun _ -> [])
-    else vrewrite ((p.cell entry).vp `vdep` mlist_cons_vp p entry (len-1) exit)
+    else vrewrite (vcell p entry `vdep` mlist_cons_vp p entry (len-1) exit)
                   (mlist_cons_sel p entry (len-1) exit)
 
-and mlist_cons_vp (p : list_param) (entry : ref p.r) (len' : nat) (exit : ref p.r) (c : t_of (p.cell entry).vp)
+and mlist_cons_vp (p : list_param) (entry : ref p.r) (len' : nat) (exit : ref p.r) (c : t_of (vcell p entry))
   : Pure vprop (requires True) (ensures fun v -> t_of v == mlist_sel_t p ((p.cell entry).get_next c) len' exit)
                (decreases %[len'; 1])
   = mlist0 p ((p.cell entry).get_next c) len' exit
@@ -36,7 +36,7 @@ let mlist_def (p : list_param) (entry : ref p.r) (len : nat) (exit : ref p.r)
   : squash (mlist0 p entry len exit ==
            (if len = 0
             then vrewrite (US.pure (entry == exit)) #(mlist_sel_t p entry len exit) (fun _ -> [])
-            else vrewrite ((p.cell entry).vp `vdep` mlist_cons_vp p entry (len-1) exit)
+            else vrewrite (vcell p entry `vdep` mlist_cons_vp p entry (len-1) exit)
                           (mlist_cons_sel p entry (len-1) exit)))
   = _ by T.(compute (); trefl ())
 
@@ -47,34 +47,34 @@ let mlist_case_O (p : list_param) (entry : ref p.r) (exit : ref p.r)
 
 let mlist_case_S (p : list_param) (entry : ref p.r) (len : nat) (exit : ref p.r)
   : Lemma (mlist0 p entry (len+1) exit ==
-           vrewrite ((p.cell entry).vp `vdep` mlist_cons_vp p entry len exit)
+           vrewrite (vcell p entry `vdep` mlist_cons_vp p entry len exit)
                     (mlist_cons_sel p entry len exit))
   = mlist_def p entry (len+1) exit
 
 let mlist_sel_case_S (p : list_param) (r0 : ref p.r) (len : nat) (exit : ref p.r) (m : Mem.mem)
   : Lemma (requires Mem.interp (hp_of (mlist0 p r0 (len+1) exit)) m)
-          (ensures  Mem.interp (hp_of (p.cell r0).vp) m /\
-                   (let c = sel_of (p.cell r0).vp m in
+          (ensures  Mem.interp (hp_of (vcell p r0)) m /\
+                   (let c = sel_of (vcell p r0) m in
                     Mem.interp (hp_of (mlist_cons_vp p r0 len exit c)) m /\
                     sel_of (mlist0 p r0 (len+1) exit) m ==
                       mlist_cons_sel p r0 len exit (|c, sel_of (mlist_cons_vp p r0 len exit c) m|)))
   =
     mlist_case_S p r0 len exit;
-    interp_vdep_hp (p.cell r0).vp (mlist_cons_vp p r0 len exit) m;
+    interp_vdep_hp (vcell p r0) (mlist_cons_vp p r0 len exit) m;
     calc (==) {
       sel_of (mlist0 p r0 (len+1) exit) m;
     == {}
-      vrewrite_sel ((p.cell r0).vp `vdep` mlist_cons_vp p r0 len exit)
+      vrewrite_sel (vcell p r0 `vdep` mlist_cons_vp p r0 len exit)
                    (mlist_cons_sel p r0 len exit) m;
-    == { vrewrite_sel_eq ((p.cell r0).vp `vdep` mlist_cons_vp p r0 len exit)
+    == { vrewrite_sel_eq (vcell p r0 `vdep` mlist_cons_vp p r0 len exit)
                          (mlist_cons_sel p r0 len exit) m }
        mlist_cons_sel p r0 len exit
          (let (|c, rs|) =
-           ((sel_of ((p.cell r0).vp `vdep` mlist_cons_vp p r0 len exit) m)
-            <: vdep_t (p.cell r0).vp (mlist_cons_vp p r0 len exit))
+           ((sel_of (vcell p r0 `vdep` mlist_cons_vp p r0 len exit) m)
+            <: vdep_t (vcell p r0) (mlist_cons_vp p r0 len exit))
           in (|c, rs|));
-    == { vdep_sel_eq (p.cell r0).vp (mlist_cons_vp p r0 len exit) m }
-     (let c = sel_of (p.cell r0).vp m in
+    == { vdep_sel_eq (vcell p r0) (mlist_cons_vp p r0 len exit) m }
+     (let c = sel_of (vcell p r0) m in
       mlist_cons_sel p r0 len exit
          (|c, sel_of (mlist_cons_vp p r0 len exit c) m|));
     }
@@ -110,15 +110,15 @@ let elim_mlist_nil_lem (p : list_param) (r0 r1 : ref p.r) (m : Mem.mem)
     US.elim_pure_lem (r0 == r1) m
 
 let intro_mlist_cons_lem (p : list_param) (r0 r1 : ref p.r) (len : nat) (exit : ref p.r) (m : Mem.mem)
-  : Lemma (requires Mem.interp (hp_of ((p.cell r0).vp `star` mlist0 p r1 len exit)) m /\
-                    (p.cell r0).get_next (sel_of (p.cell r0).vp m) == r1)
+  : Lemma (requires Mem.interp (hp_of (vcell p r0 `star` mlist0 p r1 len exit)) m /\
+                    (p.cell r0).get_next (sel_of (vcell p r0) m) == r1)
           (ensures  Mem.interp (hp_of (mlist0 p r0 (len+1) exit)) m /\
                     sel_of (mlist0 p r0 (len+1) exit) m ==
-                      (|r0, (p.cell r0).get_data (sel_of (p.cell r0).vp m)|)
+                      (|r0, (p.cell r0).get_data (sel_of (vcell p r0) m)|)
                       :: (sel_of (mlist0 p r1 len exit) m <: mlist_sel_t p r1 len exit))
   =
     mlist_case_S p r0 len exit;
-    interp_vdep_hp (p.cell r0).vp (mlist_cons_vp p r0 len exit) m;
+    interp_vdep_hp (vcell p r0) (mlist_cons_vp p r0 len exit) m;
     mlist_sel_case_S p r0 len exit m
 
 let elim_mlist_cons_lem (p : list_param) (r0 : ref p.r)
@@ -128,12 +128,12 @@ let elim_mlist_cons_lem (p : list_param) (r0 : ref p.r)
                     (sel_of (mlist0 p r0 (len + 1) exit) m
                       <: mlist_sel_t p r0 (len+1) exit) == hd :: tl)
           (ensures (let r1 = sg_entry tl exit in
-                    Mem.interp (hp_of ((p.cell r0).vp `star` mlist p r1 len exit)) m /\
-                   (let c0 = sel_of (p.cell r0).vp m in
+                    Mem.interp (hp_of (vcell p r0 `star` mlist p r1 len exit)) m /\
+                   (let c0 = sel_of (vcell p r0) m in
                     (p.cell r0).get_next c0 == r1 /\
                     (p.cell r0).get_data c0 == hd._2 /\
                     sel_of (mlist0 p r1 len exit) m == tl)))
   =
     mlist_case_S p r0 len exit;
-    interp_vdep_hp (p.cell r0).vp (mlist_cons_vp p r0 len exit) m;
+    interp_vdep_hp (vcell p r0) (mlist_cons_vp p r0 len exit) m;
     mlist_sel_case_S p r0 len exit m
