steel/Learn.Steel.ListP.Derived.fst
@@ -1,5 +1,9 @@
 module Learn.Steel.ListP.Derived
 
+module L  = FStar.List.Pure
+
+(* [mlistN] *)
+
 let v (p : list_param) (entry : ref p.r) (len : nat)
   = mlist p entry len null
 
@@ -25,3 +29,129 @@ let elim_mlistN #opened (p : list_param) entry
   =
     mlistN_indep p entry;
     US.witness_vexists (v p entry) (f p entry)
+
+
+(* append *)
+
+#push-options "--z3rlimit 10 --fuel 2 --ifuel 1" (* LONG *)
+let rec intro_mlist_append #opened p r0 (len0 : nat) r1 (len1 : nat) r2
+  =
+    let h0 = get () in
+    if len0 = 0
+    then begin
+        mlist_rew_len p r0 len0 0 r1;
+      elim_mlist_nil p r0 r1;
+      change_equal_slprop (mlist p r1 len1 r2) (mlist p r0 (len0+len1) r2);
+      let h1 = get () in
+      calc (==) {
+        sel_list p r0 (len0+len1) r2 h1
+          <: list (cell_t p);
+      == {}
+        sel_list p r1 len1 r2 h0;
+      == {}
+        L.(sel_list p r0 len0 r1 h0 @ sel_list p r1 len1 r2 h0);
+      }
+    end else begin
+      let len0' = len0 - 1 in
+        mlist_rew_len p r0 len0 (len0'+1) r1;
+      let r0' = elim_mlist_cons p r0 len0' r1 in
+      intro_mlist_append p r0' len0' r1 len1 r2;
+      intro_mlist_cons   p r0 r0' (len0'+len1) r2;
+        mlist_rew_len p r0 ((len0'+len1)+1) (len0+len1) r2;
+      let h1 = get () in
+      assert (sel_list p r0 (len0+len1) r2 h1 == L.(sel_list p r0 len0 r1 h0 @ sel_list p r1 len1 r2 h0))
+    end
+
+let rec elim_mlist_append #opened (p : list_param) r0 (len len0 len1 : nat) r2 (l0 l1 : list (cell_t p))
+  =
+    let h0 = get () in
+    calc (==) {
+      len;
+    == {}
+      L.length (sel_list p r0 len r2 h0);
+    == {}
+      L.(length (l0@l1));
+    == {}
+      len0 + len1;
+    };
+    if len0 = 0
+    then begin
+      intro_mlist_nil p r0;
+        mlist_rew_len p r0 0 len0 r0;
+        mlist_rew_len p r0 len len1 r2;
+      r0
+    end else begin
+      let hd0 :: tl0 = l0 in
+      let len'  = len  - 1 in
+      let len0' = len0 - 1 in
+        mlist_rew_len p r0 len (len'+1) r2;
+      let r0' = elim_mlist_cons p r0 len' r2 in
+      let r1  = elim_mlist_append p r0' len' len0' len1 r2 tl0 l1 in
+      intro_mlist_cons p r0 r0' len0' r1;
+        mlist_rew_len p r0 (len0'+1) len0 r1;
+      r1
+    end
+#pop-options
+
+
+(** applying ghost operations on the cells *)
+
+let mlist_extract_case_0 #opened (p : list_param) entry len exit (i : nat)
+  : SteelGhost (mlist_extract_rt p entry len exit i) opened
+      (mlist p entry len exit) (fun rt -> vcell p rt.r `star` rt.c_vp)
+      (requires fun h0 -> i = 0 /\ i < L.length (sel_list p entry len exit h0))
+      (ensures  mlist_extract_ens p entry len exit i)
+  =
+    let sl = gget (mlist p entry len exit) in
+    let len' = len - 1 in
+    mlist_rew_len p entry len (len'+1) exit;
+    let r1 = elim_mlist_cons p entry len' exit in (* TODO?: factorize with case_S *)
+    let c_sl = gget (mlist p r1 len' exit) in
+    let rt = {
+      r = entry;
+      c_vp = mlist p r1 len' exit;
+      c_sl; nxt = r1; sl;
+      close = (fun () ->
+        intro_mlist_cons p entry r1 len' exit;
+        mlist_rew_len p entry (len'+1) len exit)
+    } in
+    change_equal_slprop (vcell p entry `star` mlist p r1 len' exit)
+                        (vcell p rt.r `star` rt.c_vp);
+    rt
+
+#push-options "--z3rlimit 15"
+let rec mlist_extract_case_S #opened (p : list_param) entry len exit (i : nat)
+  : SteelGhost (mlist_extract_rt p entry len exit i) opened
+      (mlist p entry len exit) (fun rt -> vcell p rt.r `star` rt.c_vp)
+      (requires fun h0 -> i > 0 /\ i < L.length (sel_list p entry len exit h0))
+      (ensures  mlist_extract_ens p entry len exit i)
+      (decreases %[i; 0])
+  =
+    let sl = gget (mlist p entry len exit) in
+    let len' = len - 1 in
+    mlist_rew_len p entry len (len'+1) exit;
+    let r1 = elim_mlist_cons p entry len' exit in
+    let c0_sl = gget (vcell p entry) in
+    let rt' = mlist_extract p r1 len' exit (i-1) in
+    let rt  = {rt' with
+      c_vp = vcell p entry `star` rt'.c_vp;
+      c_sl = (G.reveal c0_sl, rt'.c_sl); sl;
+      close = (fun () ->
+        rt'.close ();
+        intro_mlist_cons p entry r1 len' exit;
+        mlist_rew_len p entry (len'+1) len exit)
+    } in
+    change_equal_slprop (vcell p rt'.r `star` (vcell p entry `star` rt'.c_vp))
+                        (vcell p rt.r  `star` rt.c_vp);
+    rt
+
+and mlist_extract #opened (p : list_param) entry len exit (i : nat)
+  : SteelGhost (G.erased (mlist_extract_rt p entry len exit i)) opened
+      (mlist p entry len exit) (fun rt -> vcell p rt.r `star` rt.c_vp)
+      (requires fun h0 -> i < L.length (sel_list p entry len exit h0))
+      (ensures  fun h0 rt h1 -> mlist_extract_ens p entry len exit i h0 rt h1)
+      (decreases %[i; 1])
+  = if i = 0 
+    then let rt = mlist_extract_case_0 p entry len exit i in G.hide rt
+    else let rt = mlist_extract_case_S p entry len exit i in G.hide rt
+#pop-options
