steel/Learn.Steel.Util.fst
@@ -13,39 +13,13 @@ open Steel.Reference
 
 #set-options "--ide_id_info_off"
 
-let pts_to_ref_injective_and
-      (#a:Type u#0) (r:ref a)
-      (p:perm)   (v0 v1:a) (m:mem)
-  : Lemma
-    (requires interp (pts_to_sl r p v0) m /\ interp (pts_to_sl r p v1) m)
-    (ensures  v0 == v1)
-  = pts_to_witinv r p;
-    Mem.elim_wi (pts_to_sl r p) v0 v1 m
+(* [pure] *)
 
-let noop_p (#opened) (p : vprop)
-  : SteelGhost unit opened p (fun () -> p) (fun _ -> True) (fun h0 () h1 -> frame_equalities p h0 h1)
-  = noop ()
-
-(* TODO: use? *)
-let slabsurd (#a : Type) (#opened:inames) (#p : vprop) (#q : a -> vprop) ()
-  : SteelGhost a opened p q (requires fun _ -> False) (ensures fun _ _ _ -> False)
-  = let rt : a = () in
-    change_equal_slprop p (q rt);
-    rt
-
-let rewrite_vprop #opened (#p #q : vprop) ($rw : squash (p == q))
-  : SteelGhost unit opened p (fun _ -> q)
-               (requires fun _ -> True)
-               (ensures fun h0 () h1 -> h1 q == h0 p)
-  = change_equal_slprop p q
-
-let eq_sym (#a : Type) (#x #y : a) ($p : squash (x == y)) : squash (y == x) = ()
-
-
-(* [pure] with a selector that gives a squash of the proposition *)
-
-let pure (p : prop) : vprop
+let pure0 (p : prop) : vprop
   = vrefine emp (fun _ -> p)
+
+let pure_sl  p = hp_of (pure0 p)
+let pure_sel p = reveal_emp (); sel_of (pure0 p)
 
 let intro_pure_lem (p : prop) (m : mem)
   : Lemma (requires p) (ensures interp (hp_of (pure p)) m)
@@ -60,43 +34,59 @@ let elim_pure_lem (p : prop) (m : mem)
     interp_vrefine_hp emp (fun _ -> p) m
 
 
+(* [vopt] *)
+
+let vopt0 (b : bool) (v : vprop) : vprop
+  = if b then vrewrite v #(option (t_of v)) Some
+    else vrewrite emp #(option (t_of v)) (fun _ -> None)
+
+let vopt_sl  b v = hp_of  (vopt0 b v)
+let vopt_sel b v = sel_of (vopt0 b v)
+let vopt_eq  b v : squash (vopt b v == expanded_vprop (vopt0 b v)) = ()
+
+let vopt_intro_t #opened (v : vprop)
+  : SteelGhost unit opened
+      v (fun () -> vopt true v)
+      (requires fun _ -> True) (ensures fun h0 () h1 -> h1 (vopt true v) == Some (h0 v))
+  =
+    intro_vrewrite v #(option (t_of v)) Some;
+    intro_expanded_vprop (vopt0 true v);
+    rewrite_vprop (eq_sym (vopt_eq true v))
+
+let vopt_intro_f #opened (v : vprop)
+  : SteelGhost unit opened
+      emp (fun () -> vopt false v)
+      (requires fun _ -> True) (ensures fun h0 () h1 -> h1 (vopt false v) == None)
+  =
+    intro_vrewrite emp #(option (t_of v)) (fun _ -> None);
+    assert_norm (vopt0 false v == vrewrite emp #(option (t_of v)) (fun _ -> None));
+    change_equal_slprop (vrewrite emp #(option (t_of v)) (fun _ -> None)) (vopt0 false v);
+    intro_expanded_vprop (vopt0 false v);
+    rewrite_vprop (eq_sym (vopt_eq false v))
+
+let vopt_elim_t #opened (v : vprop)
+  : SteelGhost unit opened
+      (vopt true v) (fun () -> v)
+      (requires fun _ -> True) (ensures fun h0 () h1 -> h0 (vopt true v) == Some (h1 v))
+  =
+    rewrite_vprop (vopt_eq true v);
+    elim_expanded_vprop (vopt0 true v);
+    elim_vrewrite v #(option (t_of v)) Some
+
+let vopt_elim_f #opened (v : vprop)
+  : SteelGhost unit opened
+      (vopt false v) (fun () -> emp)
+      (requires fun _ -> True) (ensures fun h0 () h1 -> h0 (vopt false v) == None)
+  =
+    rewrite_vprop (vopt_eq false v);
+    elim_expanded_vprop (vopt0 false v);
+    assert_norm (vopt0 false v == vrewrite emp #(option (t_of v)) (fun _ -> None));
+    change_equal_slprop (vopt0 false v) (vrewrite emp #(option (t_of v)) (fun _ -> None));
+    elim_vrewrite emp #(option (t_of v)) (fun _ -> None)
+
+
 (* [vexists] *)
 (* TODO? $args *)
-
-let vexists_indep (#a : Type) (v : a -> vprop) (#t : Type) (f : (x:a) -> normal (t_of (v x)) -> GTot t)
-  : Tot prop
-  = forall (x0 x1 : a) (m : mem) .
-      interp (hp_of (v x0)) m /\ interp (hp_of (v x1)) m ==>
-      f x0 (sel_of (v x0) m) == f x1 (sel_of (v x1) m)
-
-let vexists_indepD (#a : Type) (v : a -> vprop) (#t : Type) (f : (x:a) -> normal (t_of (v x)) -> GTot t) 
-                   (x0 x1 : a) (m : mem)
-  : Lemma (requires vexists_indep #a v #t f /\
-                    interp (hp_of (v x0)) m /\ interp (hp_of (v x1)) m)
-          (ensures  f x0 (sel_of (v x0) m) == f x1 (sel_of (v x1) m))
-  = ()
-
-let vexists_indepI (#a : Type) (v : a -> vprop) (#t : Type) (f : (x:a) -> normal (t_of (v x)) -> GTot t)
-  (prf : (x0 : a) -> (x1 : a) -> (m : mem) ->
-         Lemma (requires interp (hp_of (v x0)) m /\ interp (hp_of (v x1)) m)
-               (ensures  f x0 (sel_of (v x0) m) == f x1 (sel_of (v x1) m)))
-  : Lemma (ensures vexists_indep #a v #t f)
-  = 
-    introduce forall (x0 x1 : a) (m : mem) . interp (hp_of (v x0)) m /\ interp (hp_of (v x1)) m ==>
-                                        f x0 (sel_of (v x0) m) == f x1 (sel_of (v x1) m)
-      with introduce _ ==> _
-      with _ . prf x0 x1 m
-
-let vexists_indepI_unique (#a : Type) (v : a -> vprop)
-  (prf : (x0 : a) -> (x1 : a) -> (m : mem) ->
-         Lemma (requires interp (hp_of (v x0)) m /\ interp (hp_of (v x1)) m)
-               (ensures  x0 == x1))
-  : Lemma (ensures forall (t : Type) (f : (x:a) -> normal (t_of (v x)) -> GTot t)
-                   . {:pattern (vexists_indep #a v #t f)}
-                     vexists_indep #a v #t f)
-  = introduce forall t f . vexists_indep #a v #t f
-      with vexists_indepI #a v #t f prf
-
 
 let vexists_sl (#a : Type) (v : a -> vprop)
   : slprop
@@ -155,21 +145,6 @@ let vexists_sel (#a : Type) (v : a -> vprop) (#t : Type) (f : (x:a) -> normal (t
     Classical.forall_intro_2 (vexists_sel_depends_only_on      v f ());
     Classical.forall_intro   (vexists_sel_depends_only_on_core v f ());
     vexists_sel' v f
-
-[@__steel_reduce__]
-let vexists' (#a : Type) (v : a -> vprop) (#t : Type) (f : (x:a) -> normal (t_of (v x)) -> GTot t)
-  : Pure vprop' (requires vexists_indep v f) (ensures fun _ -> True)
-  = {
-    hp  = vexists_sl  v;
-    t   = t;
-    sel = vexists_sel v f
-  }
-
-[@__steel_reduce__]
-let vexists (#a : Type) (v : a -> vprop) (#t : Type) (f : (x:a) -> normal (t_of (v x)) -> GTot t)
-  : Pure vprop (requires vexists_indep v f) (ensures fun _ -> True)
-  = VUnit (vexists' v f)
-
 
 let intro_vexists_lem (#a : Type) (x : a) (v : a -> vprop)
                       (#t : Type) (f : (x:a) -> normal (t_of (v x)) -> GTot t)
@@ -237,81 +212,72 @@ let witness_vexists (#a : Type) #opened (v : a -> vprop)
     x
 
 
-(* [aptr] : abstract references *)
+(* [vdept] *)
 
-inline_for_extraction noextract noeq
-type aptr' (t : Type) = {
-  vp      : vprop;
-  of_sel  : normal (t_of vp) -> GTot t;
-  set_sel : normal (t_of vp) -> (x : t) ->
-            Ghost (normal (t_of vp)) (requires True) (ensures fun rt -> of_sel rt == x);
-  read    : unit -> Steel t vp (fun _ -> vp) (requires fun _ -> True)
-                   (ensures fun h0 x h1 -> frame_equalities vp h0 h1 /\ x == of_sel (h0 vp));
-  write   : (x : t) -> Steel unit vp (fun _ -> vp) (requires fun _ -> True)
-                   (ensures fun h0 () h1 -> h1 vp == set_sel (h0 vp) x)
-}
+let vdept0 (v : vprop) (#dt : t_of v -> Type) ($p : (x:t_of v) -> (v' : vprop {t_of v' == dt x}))
+  : Pure vprop (requires True) (ensures fun vd -> t_of vd == dtuple2 (t_of v) dt)
+  = (v `vdep` p) `vrewrite` (fun (|x, y|) -> (|x, y|) <: dtuple2 (t_of v) dt)
 
-inline_for_extraction noextract
-type aptr (t : Type) = p:aptr' t {
-     (forall (s : normal (t_of p.vp)) (x0 x1 : t) . {:pattern (p.set_sel (p.set_sel s x0) x1)}
-        p.set_sel (p.set_sel s x0) x1 == p.set_sel s x1) /\
-     (forall (s : normal (t_of p.vp)) . {:pattern (p.set_sel s (p.of_sel s))}
-        p.set_sel s (p.of_sel s) == s)
-  }
+let vdept_sl (v : vprop) (#dt : t_of v -> Type) ($p : (x:t_of v) -> (v' : vprop {t_of v' == dt x}))
+  : Mem.slprop
+  = hp_of (vdept0 v #dt p)
 
-[@@ __steel_reduce__]
-let sel_aptr (#t:Type) (#p:vprop) (x:aptr t)
-  (h:rmem p{FStar.Tactics.with_tactic selector_tactic (can_be_split p (x.vp) /\ True)})
-  : GTot (normal (t_of x.vp))
-  = h x.vp
+let vdept_sel (v : vprop) (#dt : t_of v -> Type) ($p : (x:t_of v) -> (v' : vprop {t_of v' == dt x}))
+  : selector (dtuple2 (t_of v) dt) (vdept_sl v #dt p)
+  = sel_of (vdept0 v #dt p)
 
-[@@ __steel_reduce__]
-let aptr_val (#t:Type) (#p:vprop) (x:aptr t)
-  (h:rmem p{FStar.Tactics.with_tactic selector_tactic (can_be_split p (x.vp) /\ True)})
-  : GTot t
-  = x.of_sel (h x.vp)
+let interp_vdept_sl (v : vprop) (#dt : t_of v -> Type) ($p : (x:t_of v) -> (v' : vprop {t_of v' == dt x}))
+                    (m: Mem.mem)
+  : Lemma Mem.(interp (vdept_sl v #dt p) m
+               <==> (interp (hp_of v) m /\ interp (hp_of v `star` hp_of (p (sel_of v m))) m))
+  =
+    interp_vdep_hp v p m
 
-[@@ __steel_reduce__]
-let aptr_updt (#t:Type) (#p #q:vprop) (x:aptr t) (v:t)
-  (h0:rmem p{FStar.Tactics.with_tactic selector_tactic (can_be_split p (x.vp) /\ True)})
-  (h1:rmem q{FStar.Tactics.with_tactic selector_tactic (can_be_split q (x.vp) /\ True)})
-  : prop
-  = h1 x.vp == x.set_sel (h0 x.vp) v
+let vdept_sel_eq (v : vprop) (#dt : t_of v -> Type) ($p : (x:t_of v) -> (v' : vprop {t_of v' == dt x}))
+                 (m: Mem.hmem (vdept_sl v #dt p))
+  : Lemma Mem.(
+      interp (hp_of v) m /\
+     (let x = sel_of v m in
+      interp (hp_of (p x)) m /\
+      vdept_sel v p m == (| x, sel_of (p x) m |) ))
+  =
+    vrewrite_sel_eq (v `vdep` p) (fun (|x, y|) -> (|x, y|) <: dtuple2 (t_of v) dt) m;
+    vdep_sel_eq v p m
 
+let intro_vdept (#opened:inames) (v: vprop) (q: vprop)
+                (#dt : t_of v -> Type) ($p : (x:t_of v) -> (v' : vprop {t_of v' == dt x}))
+  = change_slprop_rel_with_cond
+      (v `star` q) (vdept v #dt p)
+      (fun (vv, _) -> q == p vv)
+      (fun (vv, qv) x2 -> q == p vv /\ dfst #(t_of v) #dt x2 == vv /\ dsnd #(t_of v) #dt x2 == qv)
+      (fun m -> interp_vdept_sl v #dt p m;
+             vdept_sel_eq v #dt p m)
 
-[@@ __steel_reduce__]
-inline_for_extraction noextract
-let aptr_of_vptr (#t : Type) (r : ref t) : Tot (aptr t) = {
-  vp      = vptr r;
-  of_sel  = (fun x   -> (x <: t));
-  set_sel = (fun _ x -> x);
-  read    = (fun () -> read r);
-  write   = (fun x  -> write r x)
-}
+(* TODO: Why is it necessary ? *)
+unfold
+let rt_vp (v : vprop) (#dt : t_of v -> Type) ($p : (x:t_of v) -> (v' : vprop {t_of v' == dt x}))
+          (res : G.erased (t_of v)) : vprop
+  = v `star` p (G.reveal res)
 
+let elim_vdept (#opened:inames) (v: vprop) (#dt : t_of v -> Type) ($p : (x:t_of v) -> (v' : vprop {t_of v' == dt x}))
+: SteelGhost (G.erased (t_of v)) opened
+  (vdept v p) (fun res -> rt_vp v #dt p res)
+  (requires fun _ -> True)
+  (ensures fun h res h' ->
+      let fs = h' v in
+      let sn : dt (G.reveal res) = h' (p (G.reveal res)) in
+      let x2 = h (vdept v #dt p) in
+      G.reveal res == fs /\
+      dfst x2 == fs /\
+      dsnd x2 == sn)
+  =
+    let x2  = gget (vdept v p) in
+    let res : G.erased (t_of v) = G.hide (dfst #(t_of v) #dt x2) in
+    change_slprop_rel_with_cond
+      (vdept v p) (v `star` p (G.reveal res))
+      (fun x2' -> x2' == G.reveal x2)
+      (fun _ (vv, qv) -> vv == G.reveal res /\ qv == dsnd #(t_of v) #dt x2)
+      (fun m -> interp_vdept_sl v #dt p m;
+             vdept_sel_eq v #dt p m);
+    res
 
-inline_for_extraction noextract noeq
-type get_set_t' (c t : Type) = {
-  get : c -> Tot t;
-  set : c -> t -> Tot c;
-}
-
-inline_for_extraction noextract
-type get_set_t (c t : Type) = p:get_set_t' c t {
-     (forall (s : c) (x : t) . {:pattern (p.get (p.set s x))}
-        p.get (p.set s x) == x) /\
-     (forall (s : c) (x0 x1 : t) . {:pattern (p.set (p.set s x0) x1)}
-        p.set (p.set s x0) x1 == p.set s x1) /\
-      (forall (s : c) . {:pattern (p.set s (p.get s))}
-        p.set s (p.get s) == s)
-  }
-
-[@@ __steel_reduce__]
-inline_for_extraction noextract
-let aptr_of_get_set (#c #t : Type) ($p : get_set_t c t) (r : ref c) : Tot (aptr t) = {
-  vp      = vptr r;
-  of_sel  = (fun x   -> p.get x);
-  set_sel = (fun s x -> p.set s x);
-  read    = (fun () -> let s = read r in p.get s);
-  write   = (fun x  -> let s = read r in write r (p.set s x))
-}
