steel/Learn.Steel.Util.fsti
@@ -1,0 +1,362 @@
+module Learn.Steel.Util
+
+module G = FStar.Ghost
+module Mem = Steel.Memory
+
+open Steel.Memory
+open Steel.Effect.Common
+open Steel.Effect.Atomic
+open Steel.Effect
+open FStar.Classical.Sugar
+open Steel.FractionalPermission
+open Steel.Reference
+
+
+let pts_to_ref_injective_and
+      (#a:Type u#0) (r:ref a)
+      (p:perm)   (v0 v1:a) (m:mem)
+  : Lemma
+    (requires interp (pts_to_sl r p v0) m /\ interp (pts_to_sl r p v1) m)
+    (ensures  v0 == v1)
+  = pts_to_witinv r p;
+    Mem.elim_wi (pts_to_sl r p) v0 v1 m
+
+let noop_p (#opened) (p : vprop)
+  : SteelGhost unit opened p (fun () -> p) (fun _ -> True) (fun h0 () h1 -> frame_equalities p h0 h1)
+  = noop ()
+
+(* TODO: use? *)
+let slabsurd (#a : Type) (#opened:inames) (#p : vprop) (#q : a -> vprop) ()
+  : SteelGhost a opened p q (requires fun _ -> False) (ensures fun _ _ _ -> False)
+  = let rt : a = () in
+    change_equal_slprop p (q rt);
+    rt
+
+let rewrite_vprop #opened (#p #q : vprop) ($rw : squash (p == q))
+  : SteelGhost unit opened p (fun _ -> q)
+               (requires fun _ -> True)
+               (ensures fun h0 () h1 -> h1 q == h0 p)
+  = change_equal_slprop p q
+
+let eq_sym (#a : Type) (#x #y : a) ($p : squash (x == y)) : squash (y == x) = ()
+
+
+(* expansion of a vprop *)
+
+let expanded_vprop (v : vprop) : v':vprop{t_of v' == t_of v}
+  = VUnit ({
+    hp  = hp_of v;
+    t   = t_of v;
+    sel = sel_of v
+  })
+
+let intro_expanded_vprop_lem (v : vprop) (m : Mem.mem)
+  : Lemma (requires Mem.interp (hp_of v) m)
+          (ensures  Mem.interp (hp_of (expanded_vprop v)) m /\
+                    sel_of (expanded_vprop v) m === sel_of v m)
+  = ()
+
+let elim_expanded_vprop_lem (v : vprop) (m : Mem.mem)
+  : Lemma (requires Mem.interp (hp_of (expanded_vprop v)) m)
+          (ensures  Mem.interp (hp_of v) m /\
+                    sel_of (expanded_vprop v) m === sel_of v m)
+  = ()
+
+let intro_expanded_vprop #opened (v : vprop)
+  : SteelGhost unit opened
+               v (fun () -> expanded_vprop v)
+               (requires fun _ -> True) (ensures fun h0 _ h1 -> h1 (expanded_vprop v) == h0 v)
+  = change_slprop_rel v (expanded_vprop v)
+                      (fun sl0 sl1 -> sl1 == sl0)
+                      (intro_expanded_vprop_lem v)
+
+let elim_expanded_vprop #opened (v : vprop)
+  : SteelGhost unit opened
+               (expanded_vprop v) (fun () -> v)
+               (requires fun _ -> True) (ensures fun h0 _ h1 -> h0 (expanded_vprop v) == h1 v)
+  = change_slprop_rel (expanded_vprop v) v
+                      (fun sl0 sl1 -> sl0 == sl1)
+                      (elim_expanded_vprop_lem v)
+
+
+(* [pure] with a selector that gives a squash of the proposition *)
+
+val pure_sl  (p : prop) : Mem.slprop u#1
+val pure_sel (p : prop) : selector (squash p) (pure_sl p)
+
+[@@__steel_reduce__]
+let pure' (p : prop) : vprop' = {
+  hp  = pure_sl  p;
+  t   = squash   p;
+  sel = pure_sel p
+}
+unfold let pure (p : prop) : vprop = VUnit (pure' p)
+
+val intro_pure_lem (p : prop) (m : mem)
+  : Lemma (requires p) (ensures interp (hp_of (pure p)) m)
+
+val elim_pure_lem (p : prop) (m : mem)
+  : Lemma (requires Mem.interp (hp_of (pure p)) m) (ensures p)
+
+
+(* [vopt] *)
+
+val vopt_sl  (b : bool) (v : vprop) : Mem.slprop u#1
+val vopt_sel (b : bool) (v : vprop) : selector (option (t_of v)) (vopt_sl b v)
+
+[@@__steel_reduce__]
+let vopt' ([@@@smt_fallback] b : bool) (v : vprop) : vprop' = {
+  hp  = vopt_sl  b v;
+  t   = option (t_of v);
+  sel = vopt_sel b v
+}
+unfold let vopt ([@@@smt_fallback] b : bool) (v : vprop) : vprop = VUnit (vopt' b v)
+
+val vopt_intro_t (#opened:Mem.inames) (v : vprop)
+  : SteelGhost unit opened
+      v (fun () -> vopt true v)
+      (requires fun _ -> True) (ensures fun h0 () h1 -> h1 (vopt true v) == Some (h0 v))
+
+val vopt_intro_f (#opened:Mem.inames) (v : vprop)
+  : SteelGhost unit opened
+      emp (fun () -> vopt false v)
+      (requires fun _ -> True) (ensures fun h0 () h1 -> h1 (vopt false v) == None)
+
+val vopt_elim_t (#opened:Mem.inames) (v : vprop)
+  : SteelGhost unit opened
+      (vopt true v) (fun () -> v)
+      (requires fun _ -> True) (ensures fun h0 () h1 -> h0 (vopt true v) == Some (h1 v))
+
+val vopt_elim_f (#opened:Mem.inames) (v : vprop)
+  : SteelGhost unit opened
+      (vopt false v) (fun () -> emp)
+      (requires fun _ -> True) (ensures fun h0 () h1 -> h0 (vopt false v) == None)
+
+
+(* [vexists] *)
+(* TODO? $args *)
+
+let vexists_indep (#a : Type) (v : a -> vprop) (#t : Type) (f : (x:a) -> normal (t_of (v x)) -> GTot t)
+  : Tot prop
+  = forall (x0 x1 : a) (m : mem) .
+      interp (hp_of (v x0)) m /\ interp (hp_of (v x1)) m ==>
+      f x0 (sel_of (v x0) m) == f x1 (sel_of (v x1) m)
+
+let vexists_indepD (#a : Type) (v : a -> vprop) (#t : Type) (f : (x:a) -> normal (t_of (v x)) -> GTot t) 
+                   (x0 x1 : a) (m : mem)
+  : Lemma (requires vexists_indep #a v #t f /\
+                    interp (hp_of (v x0)) m /\ interp (hp_of (v x1)) m)
+          (ensures  f x0 (sel_of (v x0) m) == f x1 (sel_of (v x1) m))
+  = ()
+
+let vexists_indepI (#a : Type) (v : a -> vprop) (#t : Type) (f : (x:a) -> normal (t_of (v x)) -> GTot t)
+  (prf : (x0 : a) -> (x1 : a) -> (m : mem) ->
+         Lemma (requires interp (hp_of (v x0)) m /\ interp (hp_of (v x1)) m)
+               (ensures  f x0 (sel_of (v x0) m) == f x1 (sel_of (v x1) m)))
+  : Lemma (ensures vexists_indep #a v #t f)
+  = 
+    introduce forall (x0 x1 : a) (m : mem) . interp (hp_of (v x0)) m /\ interp (hp_of (v x1)) m ==>
+                                        f x0 (sel_of (v x0) m) == f x1 (sel_of (v x1) m)
+      with introduce _ ==> _
+      with _ . prf x0 x1 m
+
+let vexists_indepI_unique (#a : Type) (v : a -> vprop)
+  (prf : (x0 : a) -> (x1 : a) -> (m : mem) ->
+         Lemma (requires interp (hp_of (v x0)) m /\ interp (hp_of (v x1)) m)
+               (ensures  x0 == x1))
+  : Lemma (ensures forall (t : Type) (f : (x:a) -> normal (t_of (v x)) -> GTot t)
+                   . {:pattern (vexists_indep #a v #t f)}
+                     vexists_indep #a v #t f)
+  = introduce forall t f . vexists_indep #a v #t f
+      with vexists_indepI #a v #t f prf
+
+
+val vexists_sl (#a : Type) (v : a -> vprop)
+  : slprop u#1
+
+val vexists_sel (#a : Type) (v : a -> vprop) (#t : Type) (f : (x:a) -> normal (t_of (v x)) -> GTot t)
+  : Pure (selector t (vexists_sl #a v))
+         (requires vexists_indep v f) (ensures fun _ -> True)
+
+[@__steel_reduce__]
+let vexists' (#a : Type) (v : a -> vprop) (#t : Type) (f : (x:a) -> normal (t_of (v x)) -> GTot t)
+  : Pure vprop' (requires vexists_indep v f) (ensures fun _ -> True)
+  = {
+    hp  = vexists_sl  v;
+    t   = t;
+    sel = vexists_sel v f
+  }
+
+[@__steel_reduce__]
+let vexists (#a : Type) (v : a -> vprop) (#t : Type) (f : (x:a) -> normal (t_of (v x)) -> GTot t)
+  : Pure vprop (requires vexists_indep v f) (ensures fun _ -> True)
+  = VUnit (vexists' v f)
+
+
+val intro_vexists_lem (#a : Type) (x : a) (v : a -> vprop)
+                      (#t : Type) (f : (x:a) -> normal (t_of (v x)) -> GTot t)
+                      (m : mem)
+  : Lemma (requires vexists_indep v f /\
+                    interp (hp_of (v x)) m)
+          (ensures  interp (hp_of (vexists v f)) m /\
+                    vexists_sel v f m == f x (sel_of (v x) m))
+  
+val intro_vexists (#a : Type) (#opened:Mem.inames) (x : a) (v : a -> vprop)
+                  (#t : Type) (f : ((x:a) -> normal (t_of (v x)) -> GTot t) {vexists_indep v f})
+  : SteelGhost  unit opened
+               (v x)      (fun () -> vexists v f)
+               (fun _ -> True) (fun h0 () h1 -> h1 (vexists v f) == f x (h0 (v x)))
+
+val witness_vexists_lem (#a : Type) (v : a -> vprop)
+                        (#t : Type) (f : (x:a) -> normal (t_of (v x)) -> GTot t)
+                        (m : mem)
+  : Ghost  a
+          (requires vexists_indep v f /\
+                    interp (hp_of (vexists v f)) m)
+          (ensures fun x ->
+                    interp (hp_of (v x)) m /\
+                    vexists_sel v f m == f x (sel_of (v x) m))
+
+val witness_vexists (#a : Type) (#opened:Mem.inames) (v : a -> vprop)
+                    (#t : Type) (f : ((x:a) -> normal (t_of (v x)) -> GTot t) {vexists_indep v f})
+  : SteelGhost (G.erased a) opened
+               (vexists v f) (fun x -> v x)
+               (fun _ -> True)    (fun h0 x h1 -> h0 (vexists v f) == f x (h1 (v x)))
+
+
+(* [vdept] : [vdep] with a cast on the second component *)
+(* TODO ? use on_dom / restricted_t *)
+
+val vdept_sl (v : vprop) (#dt : t_of v -> Type) ($p : (x:t_of v) -> (v' : vprop {t_of v' == dt x}))
+  : Mem.slprop u#1
+
+val vdept_sel (v : vprop) (#dt : t_of v -> Type) ($p : (x:t_of v) -> (v' : vprop {t_of v' == dt x}))
+  : selector (dtuple2 (t_of v) dt) (vdept_sl v #dt p)
+
+[@@__steel_reduce__]
+let vdept' (v : vprop) (#dt : t_of v -> Type) ($p : (x:t_of v) -> (v' : vprop {t_of v' == dt x})) = {
+  hp  = vdept_sl  v #dt p;
+  t   = dtuple2 (t_of v) dt;
+  sel = vdept_sel v #dt p
+}
+unfold let vdept (v : vprop) (#dt : t_of v -> Type) ($p : (x:t_of v) -> (v' : vprop {t_of v' == dt x})) : vprop
+  = VUnit (vdept' v #dt p)
+
+val interp_vdept_sl (v : vprop) (#dt : t_of v -> Type) ($p : (x:t_of v) -> (v' : vprop {t_of v' == dt x}))
+                    (m: Mem.mem)
+  : Lemma Mem.(interp (vdept_sl v #dt p) m
+               <==> (interp (hp_of v) m /\ interp (hp_of v `star` hp_of (p (sel_of v m))) m))
+
+val vdept_sel_eq (v : vprop) (#dt : t_of v -> Type) ($p : (x:t_of v) -> (v' : vprop {t_of v' == dt x}))
+                 (m: Mem.hmem (vdept_sl v #dt p))
+  : Lemma Mem.(
+      interp (hp_of v) m /\
+     (let x = sel_of v m in
+      interp (hp_of (p x)) m /\
+      vdept_sel v p m == (| x, sel_of (p x) m |) ))
+
+val intro_vdept (#opened:inames) (v: vprop) (q: vprop)
+                (#dt : t_of v -> Type) ($p : (x:t_of v) -> (v' : vprop {t_of v' == dt x}))
+: SteelGhost unit opened
+    (v `star` q) (fun _ -> vdept v #dt p)
+    (requires fun h -> q == p (h v))
+    (ensures fun h _ h' ->
+      let x2 = h' (vdept v #dt p) in
+      q == p (h v) /\
+      dfst x2 == (h v) /\
+      dsnd x2 == (h q)
+    )
+
+val elim_vdept (#opened:inames) (v: vprop) (#dt : t_of v -> Type) ($p : (x:t_of v) -> (v' : vprop {t_of v' == dt x}))
+: SteelGhost (G.erased (t_of v)) opened
+  (vdept v p)
+  (fun res -> v `star` p (G.reveal res))
+  (requires fun _ -> True)
+  (ensures fun h res h' ->
+      let fs = h' v in
+      let sn : dt (G.reveal res) = h' (p (G.reveal res)) in
+      let x2 = h (vdept v #dt p) in
+      G.reveal res == fs /\
+      dfst x2 == fs /\
+      dsnd x2 == sn
+  )
+
+
+(* [aptr] : abstract references *)
+
+inline_for_extraction noextract noeq
+type aptr' (t : Type) = {
+  vp      : vprop;
+  of_sel  : normal (t_of vp) -> GTot t;
+  set_sel : normal (t_of vp) -> (x : t) ->
+            Ghost (normal (t_of vp)) (requires True) (ensures fun rt -> of_sel rt == x);
+  read    : unit -> Steel t vp (fun _ -> vp) (requires fun _ -> True)
+                   (ensures fun h0 x h1 -> frame_equalities vp h0 h1 /\ x == of_sel (h0 vp));
+  write   : (x : t) -> Steel unit vp (fun _ -> vp) (requires fun _ -> True)
+                   (ensures fun h0 () h1 -> h1 vp == set_sel (h0 vp) x)
+}
+
+inline_for_extraction noextract
+type aptr (t : Type) = p:aptr' t {
+     (forall (s : normal (t_of p.vp)) (x0 x1 : t) . {:pattern (p.set_sel (p.set_sel s x0) x1)}
+        p.set_sel (p.set_sel s x0) x1 == p.set_sel s x1) /\
+     (forall (s : normal (t_of p.vp)) . {:pattern (p.set_sel s (p.of_sel s))}
+        p.set_sel s (p.of_sel s) == s)
+  }
+
+[@@ __steel_reduce__]
+let sel_aptr (#t:Type) (#p:vprop) (x:aptr t)
+  (h:rmem p{FStar.Tactics.with_tactic selector_tactic (can_be_split p (x.vp) /\ True)})
+  : GTot (normal (t_of x.vp))
+  = h x.vp
+
+[@@ __steel_reduce__]
+let aptr_val (#t:Type) (#p:vprop) (x:aptr t)
+  (h:rmem p{FStar.Tactics.with_tactic selector_tactic (can_be_split p (x.vp) /\ True)})
+  : GTot t
+  = x.of_sel (h x.vp)
+
+[@@ __steel_reduce__]
+let aptr_updt (#t:Type) (#p #q:vprop) (x:aptr t) (v:t)
+  (h0:rmem p{FStar.Tactics.with_tactic selector_tactic (can_be_split p (x.vp) /\ True)})
+  (h1:rmem q{FStar.Tactics.with_tactic selector_tactic (can_be_split q (x.vp) /\ True)})
+  : prop
+  = h1 x.vp == x.set_sel (h0 x.vp) v
+
+
+[@@ __steel_reduce__]
+inline_for_extraction noextract
+let aptr_of_vptr (#t : Type) (r : ref t) : Tot (aptr t) = {
+  vp      = vptr r;
+  of_sel  = (fun x   -> (x <: t));
+  set_sel = (fun _ x -> x);
+  read    = (fun () -> read r);
+  write   = (fun x  -> write r x)
+}
+
+
+inline_for_extraction noextract noeq
+type get_set_t' (c t : Type) = {
+  get : c -> Tot t;
+  set : c -> t -> Tot c;
+}
+
+inline_for_extraction noextract
+type get_set_t (c t : Type) = p:get_set_t' c t {
+     (forall (s : c) (x : t) . {:pattern (p.get (p.set s x))}
+        p.get (p.set s x) == x) /\
+     (forall (s : c) (x0 x1 : t) . {:pattern (p.set (p.set s x0) x1)}
+        p.set (p.set s x0) x1 == p.set s x1) /\
+      (forall (s : c) . {:pattern (p.set s (p.get s))}
+        p.set s (p.get s) == s)
+  }
+
+[@@ __steel_reduce__]
+inline_for_extraction noextract
+let aptr_of_get_set (#c #t : Type) ($p : get_set_t c t) (r : ref c) : Tot (aptr t) = {
+  vp      = vptr r;
+  of_sel  = (fun x   -> p.get x);
+  set_sel = (fun s x -> p.set s x);
+  read    = (fun () -> let s = read r in p.get s);
+  write   = (fun x  -> let s = read r in write r (p.set s x))
+}
